src/crypto/poly1305/x64/X64.Poly1305.Math_i.fsti
@@ -1,6 +1,8 @@
 module X64.Poly1305.Math_i
 
 open FStar.Mul
+open X64.Machine_s   // needed for nat64
+open X64.Vale.Decls  // needed for shift_right64, logand64
 
 // p used to be a refinement to p > 0 and r1 a nat.
 // There are some assumptions here, which will either go away when the library switches to ints everywhere (for division too)
@@ -21,27 +23,31 @@ val lemma_poly_multiply : n:int -> p:int -> r:int -> h:int -> r0:int -> r1:int -
     hh == d2 * (n * n) + d1 * n + d0)
 	(ensures (p > 0) /\ (h * r) % p == hh % p)
 
-(*
-val lemma_poly_reduce : n:int -> p:int{ p > 0 } -> h:nat -> h2:int -> h10:int -> c:int -> hh:int -> Lemma
+// p used to be a refinement to p > 0 and h a nat.
+val lemma_poly_reduce : n:int -> p:int -> h:int -> h2:int -> h10:int -> c:int -> hh:int -> Lemma
   (requires
+    p > 0 /\
+    h >= 0 /\
+    n * n > 0 /\
+    h2 >= 0 /\  // TODO: Shouldn't need to add this
     4 * (n * n) == p + 5 /\
     h2 == h / (n * n) /\
     h10 == h % (n * n) /\
     c == (h2 / 4) + (h2 / 4) * 4 /\
     hh == h10 + c + (h2 % 4) * (n * n))
-  (ensures h % p == hh % p)
+  (ensures (p > 0) /\ (h % p == hh % p))
 
-val lemma_poly_bits64 : Lemma
+val lemma_poly_bits64 : u:unit -> Lemma
   (requires True)
   (ensures
-    (forall (x:nat64) . shift_right #64 x 2 == x / 4) /\
-    (forall (x:nat64) . shift_right #64 x 4 == x / 16) /\
-    (forall (x:nat64) . logand #64 x 3 == x % 4) /\
-    (forall (x:nat64) . logand #64 x 15 == x % 16) /\
-    (forall (x:nat64) . logand #64 x 0 == 0) /\
-    (forall (x:nat64) . logand #64 x 0xffffffffffffffff == x) /\
-    (forall (x:nat64) . logand #64 x 0xfffffffffffffffc == (x / 4) * 4) /\
-    (forall (x:nat64) . logand #64 x 0x0ffffffc0fffffff < nat64_max / 16) /\
-    (forall (x:nat64) . logand #64 x 0x0ffffffc0ffffffc < nat64_max / 16) /\
-    (forall (x:nat64) . (logand #64 x 0x0ffffffc0ffffffc) % 4 == 0))
-*)
+    (forall (x:nat64) . {:pattern (shift_right64 x 2)} shift_right64 x 2 == x / 4) /\
+    (forall (x:nat64) . {:pattern (shift_right64 x 4)} shift_right64 x 4 == x / 16) /\
+    (forall (x:nat64) . {:pattern (logand64 x 3)} logand64 x 3 == x % 4) /\
+    (forall (x:nat64) . {:pattern (logand64 x 15)} logand64 x 15 == x % 16) /\
+    (forall (x:nat64) . {:pattern (logand64 x 0)} logand64 x 0 == 0) /\
+    (forall (x:nat64) . {:pattern (logand64 x 0xffffffffffffffff)} logand64 x 0xffffffffffffffff == x) /\
+    (forall (x:nat64) . {:pattern (logand64 x 0xfffffffffffffffc)} logand64 x 0xfffffffffffffffc == (x / 4) * 4) /\
+    (forall (x:nat64) . {:pattern (logand64 x 0x0ffffffc0fffffff)} logand64 x 0x0ffffffc0fffffff < nat64_max / 16) /\
+    (forall (x:nat64) . {:pattern (logand64 x 0x0ffffffc0ffffffc)} logand64 x 0x0ffffffc0ffffffc < nat64_max / 16) /\
+    (forall (x:nat64) . {:pattern (logand64 x 0x0ffffffc0ffffffc)} (logand64 x 0x0ffffffc0ffffffc) % 4 == 0) /\
+    (forall (x:nat64)  (y:nat64) . (logand64 x y) == (logand64 y x)))
